-

Examples/BinarySearch.thy
@@ -1,17 +1,67 @@
 theory BinarySearch
-  imports "../Refine_Imperative_HOL/Sepref" "../RefineMonadicVCG"
+  imports "../Refine_Imperative_HOL/Sepref" "../RefineMonadicVCG" "SepLogicTime_RBTreeBasic.Asymptotics_1D"
 begin
 
+
+
+subsubsection "List interface"
+
+
+definition "listlookup_time = 3"
+
+context
+  fixes n::nat
+begin
+  definition "mop_lookup_list xs i = SPECT [ xs ! i \<mapsto> enat n ]"
+
+  sepref_register "mop_lookup_list" 
+  print_theorems 
+end
+
+term list_assn
+term Array.nth
+
+definition "array_assn xs p = p \<mapsto>\<^sub>a xs"
+
+lemma inst_ex_assn: "A \<Longrightarrow>\<^sub>A B x \<Longrightarrow> A \<Longrightarrow>\<^sub>A (\<exists>\<^sub>Ax. B x)"
+  using entails_ex_post by blast 
+
+lemma mop_lookup_list_as_array_rule[sepref_fr_rules]:
+  "1 \<le> n \<Longrightarrow> x < length xs \<Longrightarrow>
+    hn_refine (hn_ctxt array_assn xs p * hn_val Id x x')
+     (Array.nth p (x'::nat))
+     (hn_ctxt array_assn xs p * hn_ctxt (pure Id) x x') id_assn ( PR_CONST (mop_lookup_list n) $  xs $ x)"
+  unfolding autoref_tag_defs mop_lookup_list_def
+  apply (rule extract_cost_otherway[OF _  nth_rule, where F="nat_assn x x'"]) unfolding mult.assoc
+  unfolding hn_ctxt_def array_assn_def
+      apply(rule match_first) apply rotatel apply(rule match_first) apply (simp add: pure_def)  
+   apply(rule match_first) apply (simp add: pure_def)   apply safe 
+    apply(rule inst_ex_assn[where x="xs ! x"]) apply simp apply simp  done
+
+
+thm mop_lookup_list_as_array_rule[to_hfref]
 
 definition avg :: "nat \<Rightarrow> nat \<Rightarrow> nat" where
   "avg l r = (l + r) div 2"
 
 
 function binarysearch_time :: "nat \<Rightarrow> nat" where
-  "n < 2 \<Longrightarrow> binarysearch_time n = 2"
-| "n \<ge> 2 \<Longrightarrow> binarysearch_time n = 2 + binarysearch_time (n div 2)"
+  "n < 2 \<Longrightarrow> binarysearch_time n = 2 + listlookup_time"
+| "n \<ge> 2 \<Longrightarrow> binarysearch_time n = 2 + listlookup_time + binarysearch_time (n div 2)"
 by force simp_all
 termination by (relation "Wellfounded.measure (\<lambda>n. n)") auto
+
+definition binarysearch_time' :: "nat \<Rightarrow> real" where
+  "binarysearch_time' n = real (binarysearch_time n)"
+
+lemma div_2_to_rounding:
+  "n - n div 2 = nat \<lceil>n / 2\<rceil>" "n div 2 = nat \<lfloor>n / 2\<rfloor>" by linarith+
+
+lemma binarysearch_time'_Theta: "(\<lambda>n. binarysearch_time' n) \<in> \<Theta>(\<lambda>n. ln (real n))"
+  apply (master_theorem2 2.3 recursion: binarysearch_time.simps(2) rew: binarysearch_time'_def div_2_to_rounding)
+  unfolding listlookup_time_def
+  prefer 2 apply auto2
+  by (auto simp: binarysearch_time'_def)
 
 
 lemma binarysearch_mono:
@@ -53,22 +103,33 @@ lemma "sorted xs \<Longrightarrow> l \<le> r \<Longrightarrow> r \<le> length xs
 definition "binarysearch l r x xs =
     RECT (\<lambda>fw (l,r,x,xs).
       if l \<ge> r then RETURNT False
-    else if l + 1 \<ge> r then RETURNT (xs ! l = x)
+    else if l + 1 \<ge> r then do {
+              ASSERT (l < length xs);
+             xsi \<leftarrow> mop_lookup_list listlookup_time xs l;
+                                RETURNT (xsi = x) }
     else do {
         m \<leftarrow> RETURNT (avg l r);
-      (if xs ! m = x then RETURNT True
-      else if xs ! m < x then fw (m + 1, r, x, xs)
+        ASSERT (m < length xs);
+        xm \<leftarrow> mop_lookup_list listlookup_time xs m;
+      (if xm = x then RETURNT True
+      else if xm < x then fw (m + 1, r, x, xs)
       else fw (l, m, x, xs))
       }
   ) (l,r,x,xs)"
 
 lemma binarysearch_simps: "binarysearch l r x xs = do {
     if l \<ge> r then RETURNT False
-    else if l + 1 \<ge> r then RETURNT (xs ! l = x)
+    else if l + 1 \<ge> r then
+         do {
+              ASSERT (l < length xs);
+             xsi \<leftarrow> mop_lookup_list listlookup_time xs l;
+                                RETURNT (xsi = x) }
     else  do {
         m \<leftarrow> RETURNT (avg l r);
-      (if xs ! m = x then RETURNT True
-      else if xs ! m < x then binarysearch (m + 1) r x xs
+        ASSERT (m < length xs);
+        xm \<leftarrow> mop_lookup_list listlookup_time xs m;
+      (if xm = x then RETURNT True
+      else if xm < x then binarysearch (m + 1) r x xs
       else binarysearch l m x xs)
       } }"
   unfolding binarysearch_def by (subst RECT_unfold, refine_mono, auto)
@@ -86,17 +147,18 @@ lemma avg_between [backward] :
   "l + 1 < r \<Longrightarrow> r > avg l r"
   "l + 1 < r \<Longrightarrow> avg l r > l" by (auto simp: avg_def)
 
-lemma "sorted xs \<Longrightarrow> l \<le> r \<Longrightarrow> r \<le> length xs \<Longrightarrow>
+lemma binarysearch_correct: "sorted xs \<Longrightarrow> l \<le> r \<Longrightarrow> r \<le> length xs \<Longrightarrow>
    binarysearch l r x xs \<le> binarysearch_SPEC l r xs x"
-  unfolding binarysearch_SPEC_def
+  unfolding binarysearch_SPEC_def 
   apply(rule T_specifies_I)
 proof(induct "r-l" arbitrary: l r rule: less_induct)
   case less
   from less(2-4) show ?case
-    apply(subst binarysearch_simps) 
+    apply(subst binarysearch_simps) unfolding mop_lookup_list_def
     apply (vcg'\<open>simp\<close>)
-    apply (metis le_neq_implies_less le_refl not_less_eq) 
-    apply(rule T_conseq6) 
+            apply (metis le_neq_implies_less le_refl not_less_eq) 
+    apply(simp add: avg_def)
+    apply(rule T_conseq4)  
          apply(rule less(1)) apply (simp add: avg_def;fail)+
     subgoal 
       apply(simp only: Some_le_emb'_conv Some_eq_emb'_conv)
@@ -107,10 +169,12 @@ proof(induct "r-l" arbitrary: l r rule: less_induct)
       done
     subgoal 
       using le_less_Suc_eq by fastforce 
+    apply(simp add: avg_def)
     subgoal by auto2    (* <<<<<<<<<<<<<<<<<<<<<<<<<<<  :) *)
     subgoal 
       using le_less_Suc_eq by fastforce 
-    apply(rule T_conseq6) 
+    apply(simp add: avg_def)
+    apply(rule T_conseq4) 
          apply(rule less(1)) apply (simp add: avg_def;fail)+
     subgoal 
       apply(simp only: Some_le_emb'_conv Some_eq_emb'_conv)
@@ -124,6 +188,65 @@ qed
 
    
 
+context 
+  fixes l::"nat"
+  notes [[sepref_register_adhoc l]]
+  notes [sepref_import_param] = IdI[of l] 
+  fixes r::"nat"
+  notes [[sepref_register_adhoc r]]
+  notes [sepref_import_param] = IdI[of r] 
+  fixes x::"nat"
+  notes [[sepref_register_adhoc x]]
+  notes [sepref_import_param] = IdI[of x] 
+begin 
+
+declare listlookup_time_def [simp]
+
+sepref_definition binarysearch_impl is "(binarysearch l r x)" :: "array_assn\<^sup>k \<rightarrow>\<^sub>a bool_assn"
+  unfolding binarysearch_def avg_def 
+  using [[goals_limit = 3]] 
+
+  apply sepref_dbg_preproc
+  apply sepref_dbg_cons_init
+  apply sepref_dbg_id 
+     apply sepref_dbg_monadify
+
+     apply sepref_dbg_opt_init
+
+  thm sepref_fr_rules     
+  thm sepref_comb_rules          
+
+  apply sepref_dbg_trans_step+ 
+
+
+  apply sepref_dbg_opt
+  apply sepref_dbg_cons_solve \<comment> \<open>Frame rule, recovering the invalidated list 
+    or pure elements, propagating recovery over the list structure\<close>
+  apply sepref_dbg_cons_solve \<comment> \<open>Trivial frame rule\<close>
+  apply sepref_dbg_constraints 
+  sorry
+ 
+
+thm binarysearch_impl.refine[to_hnr]
+thm hnr_refine[OF binarysearch_correct ] binarysearch_impl.refine[to_hnr, unfolded autoref_tag_defs]
+thm  hnr_refine[OF binarysearch_correct, OF _ _ _ binarysearch_impl.refine[to_hnr, unfolded autoref_tag_defs]] 
+
+lemma binary_search_impl_correct: "sorted xs \<Longrightarrow> l \<le> r \<Longrightarrow> r \<le> length xs \<Longrightarrow> hn_refine (hn_ctxt array_assn xs p) (binarysearch_impl p) (hn_ctxt array_assn xs p) bool_assn (binarysearch_SPEC l r xs x)"
+  using hnr_refine[OF binarysearch_correct, OF _ _ _ binarysearch_impl.refine[to_hnr, unfolded autoref_tag_defs]]  by auto 
+
+thm extract_cost_ub'[OF binary_search_impl_correct[unfolded  binarysearch_SPEC_def], where Cost_ub="binarysearch_time (r - l)" ]
+lemma "sorted xs \<Longrightarrow> r \<le> length xs \<Longrightarrow> l \<le> r \<Longrightarrow> 
+     <hn_ctxt array_assn xs p * timeCredit_assn (binarysearch_time (r - l))> 
+        binarysearch_impl p
+       <\<lambda>ra. hn_ctxt array_assn xs p * \<up> (ra \<longleftrightarrow> (\<exists>i\<ge>l. i < r \<and> xs ! i = x))>\<^sub>t"
+  apply(rule extract_cost_ub'[OF binary_search_impl_correct[unfolded  binarysearch_SPEC_def], where Cost_ub="binarysearch_time (r - l)" ])
+       apply auto
+     apply(subst in_ran_emb_special_case) apply (simp_all add: pure_def) apply auto
+   by (metis (no_types, lifting) ent_true_drop(1) entails_ex entt_refl') 
+
+
+lemma "binarysearch_time \<in> \<Theta>(\<lambda>n. ln (real n))"
+  using binarysearch_time'_Theta unfolding binarysearch_time'_def by auto
 
 
 
