RefineMonadicVCG.thy
@@ -63,4 +63,22 @@ lemma progress_bind[progress_rules]: "progress m \<or> (\<forall>x. progress (f 
 
 
 
+
+
+lemma ran_emb': "c \<in> ran (emb' Q t) \<longleftrightarrow> (\<exists>s'. Q s' \<and> t s' = c)"
+  by(auto simp: emb'_def ran_def)
+
+lemma ran_emb_conv: "Ex Q \<Longrightarrow>  ran (emb Q t) = {t}"
+  by (auto simp: ran_emb')
+
+lemma in_ran_emb_special_case: "c\<in>ran (emb Q t) \<Longrightarrow> c\<le>t"
+  apply (cases "Ex Q")
+   apply (auto simp: ran_emb_conv)
+  apply (auto simp: emb'_def)
+  done
+
+lemma dom_emb'_eq[simp]: "dom (emb' Q f) = Collect Q"
+  by(auto simp: emb'_def split: if_splits)
+
+
 end
